Verification/VerificationCDPC.dfy
@@ -4,6 +4,8 @@ include "../Auxiliary/Lemmas.dfy"
 include "../Auxiliary/Set.dfy"
 include "../Auxiliary/Map.dfy"
 include "../Auxiliary/Interview.dfy"
+include "../Verification/VerificationCDPC_aux.dfy"
+
 
 method verifyCDPC(f:Map_Map_T<int, bool, bool>, g:Map_Map_T<int, bool, int>, P:Set<int>, a:real, b:real, x:real, y:real, iv:Interview) returns (r:bool, ghost counter:nat)
   requires pred_problem_preconditions(f, g, P, a, b, x, y, iv)
@@ -18,8 +20,8 @@ method verifyCDPC(f:Map_Map_T<int, bool, bool>, g:Map_Map_T<int, bool, int>, P:S
   return r, counter;
 }
 
-method {:only} verifyCDPC_rec(f:Map_Map_T<int, bool, bool>, g:Map_Map_T<int, bool, int>, P:Set<int>, a:real, b:real, x:real, y:real, iv:Interview, ghost nodes:nat, ghost counter_in:nat) returns (r:bool, ghost counter:nat)
-  decreases nodes // iv.Questions()
+method verifyCDPC_rec(f:Map_Map_T<int, bool, bool>, g:Map_Map_T<int, bool, int>, P:Set<int>, a:real, b:real, x:real, y:real, iv:Interview, ghost nodes:nat, ghost counter_in:nat) returns (r:bool, ghost counter:nat)
+  decreases nodes
   requires pred_problem_preconditions(f, g, P, a, b, x, y, iv)
   requires pred_nodes(iv, f, nodes)
   ensures reveal pred_problem_preconditions(f, g, P, a, b, x, y, iv); r == certificateCDPC(f.Model(), g.Model(), P.Model(), a, b, x, y, iv.Model())
@@ -83,46 +85,96 @@ method {:only} verifyCDPC_rec(f:Map_Map_T<int, bool, bool>, g:Map_Map_T<int, boo
       ghost var nodes_true := |iv_true.Questions()|*f_true.Cardinality() + 1;
       ghost var nodes_false := |iv_false.Questions()|*f_false.Cardinality() + 1;
 
-      r, counter := verifyCDPC_inductive_step(f, g, P, a, b, x, y, iv,
-                                 f_true, g_true, iv_true,
-                                 f_false, g_false, iv_false,
-                                 question, question_is_valid_and_not_trivial, nodes_true, nodes_false,
-                                 nodes, counter_in)
-      by {
-        assert (nodes_true < nodes) && (nodes_false < nodes) by {
+      var recursive_true:bool; recursive_true, counter := verifyCDPC_rec(f_true, g_true, P, a, b, x, y, iv_true, nodes_true, counter) by {
+        reveal pred_problem_preconditions(f, g, P, a, b, x, y, iv);
+        reveal pred_branch_info(iv, question_is_valid_and_not_trivial, question);
+        reveal pred_variables_inductive_step(f, g, P, a, b, x, y, iv, question, question_is_valid_and_not_trivial, f_true, g_true, iv_true, nodes_true, f_false, g_false, iv_false, nodes_false);
+        reveal pred_nodes(iv_true, nodes_true);
+        assert 0 < nodes_true by {
+          assert (exists c:candidate | c in f.Keys() :: c[question] == true);
+          ghost var cand_true :| cand_true in f.Keys() && cand_true[question] == true;
+          assert f_true.Model() == (map c:candidate | c in f.Keys() && c[question] == true :: f.Model()[c]);
+          assert cand_true in f_true.Model();
+          assert 1 <= f_true.Cardinality();
+          assert 0 <= |iv_true.Questions()|;
+          mult_preserves_order(0, 1, |iv_true.Questions()|, f_true.Cardinality());
+        }
+        assert nodes_true < nodes by {
           reveal pred_nodes(iv, f, nodes);
           mult_preserves_strict_order(|iv_true.Questions()|, f_true.Cardinality(), |iv.Questions()|, f.Cardinality());
+        }
+      }
+      var recursive_false:bool; recursive_false, counter := verifyCDPC_rec(f_false, g_false, P, a, b, x, y, iv_false, nodes_false, counter) by {
+        reveal pred_problem_preconditions(f, g, P, a, b, x, y, iv);
+        reveal pred_branch_info(iv, question_is_valid_and_not_trivial, question);
+        reveal pred_variables_inductive_step(f, g, P, a, b, x, y, iv, question, question_is_valid_and_not_trivial, f_true, g_true, iv_true, nodes_true, f_false, g_false, iv_false, nodes_false);
+        reveal pred_nodes(iv_true, nodes_true);
+        assert 0 < nodes_false  by {
+          assert (exists c:candidate | c in f.Keys() :: c[question] == false);
+          ghost var cand_false :| cand_false in f.Keys() && cand_false[question] == false;
+          assert f_false.Model() == (map c:candidate | c in f.Keys() && c[question] == false :: f.Model()[c]);
+          assert cand_false in f_false.Model();
+          assert 1 <= f_false.Cardinality();
+          assert 0 <= |iv_false.Questions()|;
+          mult_preserves_order(0, 1, |iv_false.Questions()|, f_false.Cardinality());
+        }
+        assert nodes_false < nodes by {
+          reveal pred_nodes(iv, f, nodes);
           mult_preserves_strict_order(|iv_false.Questions()|, f_false.Cardinality(), |iv.Questions()|, f.Cardinality());
         }
-        assert pred_problem_preconditions(f, g, P, a, b, x, y, iv);
-        assert pred_branch_info(iv, question_is_valid_and_not_trivial, question) by { reveal pred_branch_info(); }
-        assume false;
-        assert pred_variables_inductive_step(f, g, P, a, b, x, y, iv, question, question_is_valid_and_not_trivial, f_true, g_true, iv_true, nodes_true, f_false, g_false, iv_false, nodes_false);
+      }
+      r := question_is_valid_and_not_trivial && recursive_true && recursive_false;
+      assert counter <= counter_in + poly_verifyCDPC_node(f, g, P, iv) + nodes_true*poly_verifyCDPC_node(f_true, g_true, P, iv_true) + nodes_false*poly_verifyCDPC_node(f_false, g_false, P, iv_false);
+      
+      assert
+          (recursive_true == certificateCDPC(
+          (map c:candidate | c in f.Keys() && c[question] == true :: f.Model()[c]),
+          (map c:candidate | c in g.Keys() && c[question] == true :: g.Model()[c]),
+          P.Model(), a, b, x, y, iv.Model().True
+        ))
+        &&
+        (recursive_false == certificateCDPC(
+          (map c:candidate | c in f.Keys() && c[question] == false :: f.Model()[c]),
+          (map c:candidate | c in g.Keys() && c[question] == false :: g.Model()[c]),
+          P.Model(), a, b, x, y, iv.Model().False
+        ))
+      by {
+        reveal pred_problem_preconditions(f, g, P, a, b, x, y, iv);
+        reveal pred_branch_info(iv, question_is_valid_and_not_trivial, question);
+        reveal pred_variables_inductive_step(f, g, P, a, b, x, y, iv, question, question_is_valid_and_not_trivial, f_true, g_true, iv_true, nodes_true, f_false, g_false, iv_false, nodes_false);
+      }
+
+      postcondition_verifyCDPC(f, g, P, a, b, x, y, iv, question, question_is_valid_and_not_trivial, recursive_true, recursive_false, r) by {
+        assert pred_variables_lemma(f, g, P, a, b, x, y, iv, question, question_is_valid_and_not_trivial, recursive_true, recursive_false, r) by {
+          reveal pred_variables_lemma(f, g, P, a, b, x, y, iv, question, question_is_valid_and_not_trivial, recursive_true, recursive_false, r);
+          reveal pred_branch_info(iv, question_is_valid_and_not_trivial, question);
+          reveal pred_variables_inductive_step(f, g, P, a, b, x, y, iv, question, question_is_valid_and_not_trivial, f_true, g_true, iv_true, nodes_true, f_false, g_false, iv_false, nodes_false);
+        }
       }
       
       assert counter <= counter_in + nodes*poly_verifyCDPC_node(f, g, P, iv) by {
-        assert counter <= counter_in + poly_verifyCDPC_node(f_true, g_true, P, iv_true) + nodes_true*poly_verifyCDPC_node(f_true, g_true, P, iv_true) + nodes_false*poly_verifyCDPC_node(f_false, g_false, P, iv_false);
-        assert counter <= counter_in + (nodes_true + nodes_false + 1)*poly_verifyCDPC_node(f_false, g_false, P, iv_false);
-        assert (nodes_true + nodes_false + 1) <= nodes by {
-          reveal pred_nodes(iv, f, nodes);
-          assert nodes == |iv.Questions()|*f.Cardinality() + 1;
-          assert nodes_true == |iv_true.Questions()|*f_true.Cardinality() + 1;
-          assert nodes_false == |iv_false.Questions()|*f_false.Cardinality() + 1;
-          assert (|iv_true.Questions()| < |iv.Questions()|) && (|iv_false.Questions()| < |iv.Questions()|);
-          assert f_true.Cardinality() + f_false.Cardinality() == f.Cardinality();
-
-          ghost var Q := |iv.Questions()|;
-          ghost var C := f.Cardinality();
-          ghost var A := C - f_true.Cardinality();
-          
-          assert nodes == Q*C + 1;
-          assert nodes_true <= (Q - 1)*(C - A) + 1;
-          assert nodes_false <= (Q - 1)*(A) + 1;
-
-          assume false;
+        reveal pred_nodes(iv, f, nodes);
+        assert f_true.Cardinality() + f_false.Cardinality() == f.Cardinality() by {
+          reveal pred_problem_preconditions(f, g, P, a, b, x, y, iv);
+          candidates_with_same_answer_lemma(f, f_true, f_false, question);
         }
+        assert 0 < f_true.Cardinality() by {
+          assert (exists c:candidate | c in f.Keys() :: c[question] == true);
+          ghost var cand_true :| cand_true in f.Keys() && cand_true[question] == true;
+          assert f_true.Model() == (map c:candidate | c in f.Keys() && c[question] == true :: f.Model()[c]);
+          assert cand_true in f_true.Model();
+          assert 1 <= f_true.Cardinality();
+        }
+        assert 0 < f_false.Cardinality() by {
+          assert (exists c:candidate | c in f.Keys() :: c[question] == false);
+          ghost var cand_false :| cand_false in f.Keys() && cand_false[question] == false;
+          assert f_false.Model() == (map c:candidate | c in f.Keys() && c[question] == false :: f.Model()[c]);
+          assert cand_false in f_false.Model();
+          assert 1 <= f_false.Cardinality();
+        }
+        verifyCDPC_restore_counter(f, g, P, iv, nodes, f_true, f_false, g_true, g_false, nodes_true, nodes_false, iv_true, iv_false, counter, counter_in);
       }
-
+      
       return r, counter;
     }
 
@@ -136,88 +188,6 @@ method {:only} verifyCDPC_rec(f:Map_Map_T<int, bool, bool>, g:Map_Map_T<int, boo
     return false, counter;
   }
 }
-
-
-method {:only} verifyCDPC_inductive_step(f:Map_Map_T<int, bool, bool>, g:Map_Map_T<int, bool, int>, P:Set<int>, a:real, b:real, x:real, y:real, iv:Interview,
-                                 f_true:Map_Map_T<int, bool, bool>, g_true:Map_Map_T<int, bool, int>, iv_true:Interview,
-                                 f_false:Map_Map_T<int, bool, bool>, g_false:Map_Map_T<int, bool, int>, iv_false:Interview,
-                                 question:int, question_is_valid_and_not_trivial:bool, ghost nodes_true:nat, ghost nodes_false:nat,
-                                 ghost nodes:nat, ghost counter_in:nat)
-                                 returns (r:bool, ghost counter:nat)
-  decreases reveal pred_variables_inductive_step(f, g, P, a, b, x, y, iv, question, question_is_valid_and_not_trivial, f_true, g_true, iv_true, nodes_true, f_false, g_false, iv_false, nodes_false); nodes
-  requires (nodes_true < nodes) && (nodes_false < nodes)
-
-  requires pred_problem_preconditions(f, g, P, a, b, x, y, iv)
-  requires pred_branch_info(iv, question_is_valid_and_not_trivial, question)
-  requires pred_variables_inductive_step(f, g, P, a, b, x, y, iv, question, question_is_valid_and_not_trivial, f_true, g_true, iv_true, nodes_true, f_false, g_false, iv_false, nodes_false)
-
-  ensures reveal pred_problem_preconditions(f, g, P, a, b, x, y, iv); r == certificateCDPC(f.Model(), g.Model(), P.Model(), a, b, x, y, iv.Model())
-  ensures counter <= counter_in + nodes_true*poly_verifyCDPC_node(f_true, g_true, P, iv_true) + nodes_false*poly_verifyCDPC_node(f_false, g_false, P, iv_false)
-{
-  counter := counter_in;
-  var recursive_true:bool; recursive_true, counter := verifyCDPC_rec(f_true, g_true, P, a, b, x, y, iv_true, nodes_true, counter) by {
-    reveal pred_problem_preconditions(f, g, P, a, b, x, y, iv);
-    reveal pred_branch_info(iv, question_is_valid_and_not_trivial, question);
-    reveal pred_variables_inductive_step(f, g, P, a, b, x, y, iv, question, question_is_valid_and_not_trivial, f_true, g_true, iv_true, nodes_true, f_false, g_false, iv_false, nodes_false);
-    reveal pred_nodes(iv_true, nodes_true);
-    assert 0 < nodes_true by {
-      assert (exists c:candidate | c in f.Keys() :: c[question] == true);
-      ghost var cand_true :| cand_true in f.Keys() && cand_true[question] == true;
-      assert f_true.Model() == (map c:candidate | c in f.Keys() && c[question] == true :: f.Model()[c]);
-      assert cand_true in f_true.Model();
-      assert 1 <= f_true.Cardinality();
-      assert 0 <= |iv_true.Questions()|;
-      mult_preserves_order(0, 1, |iv_true.Questions()|, f_true.Cardinality());
-    }
-    assert nodes_true < nodes;
-  }
-  var recursive_false:bool; recursive_false, counter := verifyCDPC_rec(f_false, g_false, P, a, b, x, y, iv_false, nodes_false, counter) by {
-    reveal pred_problem_preconditions(f, g, P, a, b, x, y, iv);
-    reveal pred_branch_info(iv, question_is_valid_and_not_trivial, question);
-    reveal pred_variables_inductive_step(f, g, P, a, b, x, y, iv, question, question_is_valid_and_not_trivial, f_true, g_true, iv_true, nodes_true, f_false, g_false, iv_false, nodes_false);
-    reveal pred_nodes(iv_true, nodes_true);
-    assert 0 < nodes_false  by {
-      assert (exists c:candidate | c in f.Keys() :: c[question] == false);
-      ghost var cand_false :| cand_false in f.Keys() && cand_false[question] == false;
-      assert f_false.Model() == (map c:candidate | c in f.Keys() && c[question] == false :: f.Model()[c]);
-      assert cand_false in f_false.Model();
-      assert 1 <= f_false.Cardinality();
-      assert 0 <= |iv_false.Questions()|;
-      mult_preserves_order(0, 1, |iv_false.Questions()|, f_false.Cardinality());
-    }
-  }
-  r := question_is_valid_and_not_trivial && recursive_true && recursive_false;
-  assert counter <= counter_in + poly_verifyCDPC_node(f, g, P, iv) + nodes_true*poly_verifyCDPC_node(f_true, g_true, P, iv_true) + nodes_false*poly_verifyCDPC_node(f_false, g_false, P, iv_false);
-  
-  assert
-      (recursive_true == certificateCDPC(
-      (map c:candidate | c in f.Keys() && c[question] == true :: f.Model()[c]),
-      (map c:candidate | c in g.Keys() && c[question] == true :: g.Model()[c]),
-      P.Model(), a, b, x, y, iv.Model().True
-    ))
-    &&
-    (recursive_false == certificateCDPC(
-      (map c:candidate | c in f.Keys() && c[question] == false :: f.Model()[c]),
-      (map c:candidate | c in g.Keys() && c[question] == false :: g.Model()[c]),
-      P.Model(), a, b, x, y, iv.Model().False
-    ))
-  by {
-    reveal pred_problem_preconditions(f, g, P, a, b, x, y, iv);
-    reveal pred_branch_info(iv, question_is_valid_and_not_trivial, question);
-    reveal pred_variables_inductive_step(f, g, P, a, b, x, y, iv, question, question_is_valid_and_not_trivial, f_true, g_true, iv_true, nodes_true, f_false, g_false, iv_false, nodes_false);
-  }
-
-  postcondition_verifyCDPC(f, g, P, a, b, x, y, iv, question, question_is_valid_and_not_trivial, recursive_true, recursive_false, r) by {
-    assert pred_variables_lemma(f, g, P, a, b, x, y, iv, question, question_is_valid_and_not_trivial, recursive_true, recursive_false, r) by {
-      reveal pred_variables_lemma(f, g, P, a, b, x, y, iv, question, question_is_valid_and_not_trivial, recursive_true, recursive_false, r);
-      reveal pred_branch_info(iv, question_is_valid_and_not_trivial, question);
-      reveal pred_variables_inductive_step(f, g, P, a, b, x, y, iv, question, question_is_valid_and_not_trivial, f_true, g_true, iv_true, nodes_true, f_false, g_false, iv_false, nodes_false);
-    }
-  }
-
-  return r, counter;
-}
-
 
 
 method verifyCDPC_base_case(f:Map_Map_T<int, bool, bool>, g:Map_Map_T<int, bool, int>, P:Set<int>, a:real, b:real, x:real, y:real, iv:Interview, ghost nodes:nat, ghost counter_in:nat) returns (r:bool, ghost counter:nat)
@@ -496,8 +466,13 @@ method correct_private_ratio_inner_loop(f:Map_Map_T<int, bool, bool>, f'_in:Map_
   }
 
   assert numPriv == |(set privCand:candidate | privCand in (f.Keys() - f'.Keys()) && privCand[p] :: privCand)| by {
-    assert f'_in.Keys() == (f'.Keys() + {cand.Model()});
-    assert (f.Keys() - (f'.Keys() + {cand.Model()})) == (f.Keys() -f'.Keys() - {cand.Model()});
+    assert f'_in.Keys() == (f'.Keys() + {cand.Model()}) by {
+      assert f'.Keys() == f'_in.Keys() - {cand.Model()};
+      set_operation_swap_sign_addition(f'_in.Keys(), f'.Keys(), cand.Model());
+    }
+    assert (f.Keys() - (f'.Keys() + {cand.Model()})) == (f.Keys() - f'.Keys() - {cand.Model()}) by {
+      set_operation_remove_parenthesis(f.Keys(), f'.Keys(), cand.Model());
+    }
     assert if isPrivate then numPriv == |(set privCand:candidate | privCand in (f.Keys() - f'.Keys() - {cand.Model()}) && privCand[p] :: privCand)| + 1
             else           numPriv == |(set privCand:candidate | privCand in (f.Keys() - f'.Keys() - {cand.Model()}) && privCand[p] :: privCand)|;
     lemma_card_priv_set_when_remove_element(f.Model(), f.Keys() - f'.Keys(), cand.Model(), p);
@@ -515,12 +490,13 @@ method candidates_with_same_answer<T>(f:Map_Map_T<int, bool, T>, question:int, a
   requires f.Valid()
   requires forall c1, c2:candidate |  c1 in f.Keys() && c2 in f.Keys() :: c1.Keys == c2.Keys
   requires forall c:candidate |  c in f.Keys() :: question in c
-  //requires (exists cand:candidate | cand in f.Keys() :: cand[question] == true)
-  //requires (exists cand:candidate | cand in f.Keys() :: cand[question] == false)
+
   ensures f_out.Valid()
   ensures f_out.Model() == (map c:candidate | c in f.Keys() && c[question] == answer :: f.Model()[c])
+  ensures f_out.UBSize() <= f.UBSize()
   ensures f_out.Cardinality() <= f.Cardinality()
-  //ensures 0 < f_out.Cardinality()
+  ensures f_out.UBSize_Keys() <= f.UBSize_Keys()
+
   ensures counter <= counter_in + poly_candidates_with_same_answer(f)
 {
   counter := counter_in;
@@ -543,6 +519,7 @@ method candidates_with_same_answer<T>(f:Map_Map_T<int, bool, T>, question:int, a
     invariant f'Empty == (f'.Cardinality() == 0)
     invariant f_out.Model() == (map c:candidate | c in (f.Keys() - f'.Keys()) && c[question] == answer :: f.Model()[c])
     invariant f_out.Cardinality() <= (f.Cardinality() - f'.Cardinality())
+    invariant f_out.UBSize_Keys() <= f.UBSize_Keys()
     invariant counter <= counter_in + f.UBSize() + 2 + (f.Cardinality() - f'.Cardinality())*poly_candidates_with_same_answer_loop(f)
     invariant f'Empty == (f'.Cardinality() == 0)
   {
@@ -552,6 +529,7 @@ method candidates_with_same_answer<T>(f:Map_Map_T<int, bool, T>, question:int, a
   }
   identity_substraction_lemma(f.Keys(), f'.Keys());
   candidates_with_same_answer_counter_simplification(f, f', counter, counter_in);
+  in_universe_lemma_Map_Map_T(f_out, f);
   assert counter <= counter_in + poly_candidates_with_same_answer(f);
 
   return f_out, counter;
@@ -567,6 +545,7 @@ method candidates_with_same_answer_loop<T>(f:Map_Map_T<int, bool, T>, f'_in:Map_
   requires f'_in.Cardinality() != 0
   requires f''_in.Model() == (map c:candidate | c in (f.Keys() - f'_in.Keys()) && c[question] == answer :: f.Model()[c])
   requires f''_in.Cardinality() <= (f.Cardinality() - f'_in.Cardinality())
+  requires f''_in.UBSize_Keys() <= f.UBSize_Keys()
 
   ensures f'.Cardinality() == f'_in.Cardinality() - 1
 
@@ -576,6 +555,7 @@ method candidates_with_same_answer_loop<T>(f:Map_Map_T<int, bool, T>, f'_in:Map_
   
   ensures f''.Model() == (map c:candidate | c in (f.Keys() - f'.Keys()) && c[question] == answer :: f.Model()[c])
   ensures f''.Cardinality() <= (f.Cardinality() - f'.Cardinality())
+  ensures f''.UBSize_Keys() <= f.UBSize_Keys()
   ensures counter <= counter_in + poly_candidates_with_same_answer_loop(f)
 {
   in_universe_lemma_Map_Map_T(f'_in, f);
@@ -586,13 +566,13 @@ method candidates_with_same_answer_loop<T>(f:Map_Map_T<int, bool, T>, f'_in:Map_
   f', counter := f'_in.Remove(cand, counter);
 
   var cand_answer:bool; cand_answer, counter := cand.Get(question, counter);
-
+  
   if (cand_answer == answer) {
     var f_cand:T; f_cand, counter := f.Get(cand, counter);
     f'', counter := f''_in.Insert(cand, f_cand, counter);
 
     assert (forall k | k in f''_in.Universe().Keys :: f''.Universe()[k] == f.Universe()[k]);
-    candidates_with_same_answer_lemma_1<T>(f, f'_in, f''_in, f', f'', cand, question, answer);
+    candidates_with_same_answer_lemma_1(f, f'_in, f''_in, f', f'', cand, question, answer);
   }
   else {
     f'', counter := f''_in.Copy(counter);
@@ -605,450 +585,126 @@ method candidates_with_same_answer_loop<T>(f:Map_Map_T<int, bool, T>, f'_in:Map_
 }
 
 
+/*
 
+  ...
 
-// POLYNOMIALS
+  r, counter := verifyCDPC_inductive_step(f, g, P, a, b, x, y, iv,
+                                          f_true, g_true, iv_true,
+                                          f_false, g_false, iv_false,
+                                          question, question_is_valid_and_not_trivial, nodes_true, nodes_false,
+                                          nodes, counter_in)
+  by {
+    assert (nodes_true < nodes) && (nodes_false < nodes) by {
+      reveal pred_nodes(iv, f, nodes);
+      mult_preserves_strict_order(|iv_true.Questions()|, f_true.Cardinality(), |iv.Questions()|, f.Cardinality());
+      mult_preserves_strict_order(|iv_false.Questions()|, f_false.Cardinality(), |iv.Questions()|, f.Cardinality());
+    }
+    assert pred_problem_preconditions(f, g, P, a, b, x, y, iv);
+    assert pred_branch_info(iv, question_is_valid_and_not_trivial, question) by { reveal pred_branch_info(); }
+    
+    assert (f_true.Valid() && f_false.Valid() && g_true.Valid() && g_false.Valid() && iv_true.Valid() && iv_false.Valid());
+    assert (question_is_valid_and_not_trivial == (
+      (forall cand:candidate | cand in f.Keys() :: question in cand.Keys) &&    // candidates have question
+      (exists cand:candidate | cand in f.Keys() :: cand[question] == true) &&   // exists answer true
+      (exists cand:candidate | cand in f.Keys() :: cand[question] == false))    // exists answer false
+    );
+    assert ((iv_true.Model() == iv.Model().True) && iv_true.Questions() == iv.Questions() - {iv.Model().Key});
+    assert ((iv_false.Model() == iv.Model().False) && iv_false.Questions() == iv.Questions() - {iv.Model().Key});
+    assert (nodes_true == |iv_true.Questions()|*f_true.Cardinality() + 1);
+    assert (nodes_false == |iv_false.Questions()|*f_false.Cardinality() + 1);
+    
+    assert (f_true.Model() == (map c:candidate | c in f.Keys() && c[question] == true :: f.Model()[c]));
+    assert (f_false.Model() == (map c:candidate | c in f.Keys() && c[question] == false :: f.Model()[c]));
+    assert (g_true.Model() == (map c:candidate | c in g.Keys() && c[question] == true :: g.Model()[c]));
+    assert (g_false.Model() == (map c:candidate | c in g.Keys() && c[question] == false :: g.Model()[c]));
+    assert false;
 
-
-ghost opaque function poly_verifyCDPC(f:Map_Map_T<int, bool, bool>, g:Map_Map_T<int, bool, int>, P:Set<int>, iv:Interview) : (o:nat)
-{
-  (|iv.Questions()|*f.Cardinality() + 1)*poly_verifyCDPC_node(f, g, P, iv)
-}
-
-ghost opaque function poly_verifyCDPC_node(f:Map_Map_T<int, bool, bool>, g:Map_Map_T<int, bool, int>, P:Set<int>, iv:Interview) : (o:nat)
-  ensures poly_verifyCDPC_base_case(f, g, P, iv) + 1 <= o
-  ensures f.UBSize() + 3 + f.Cardinality()*poly_loop_check_that_candidates_have_question_and_that_it_isnt_trivial(f) <= o
-  ensures f.UBSize() + 3 + f.Cardinality()*poly_loop_check_that_candidates_have_question_and_that_it_isnt_trivial(f) + 2*poly_candidates_with_same_answer(f) + 2*poly_candidates_with_same_answer(g) + 2*iv.UBSize() <= o
-{
-  calc <= {
-    f.UBSize() + 3 + f.Cardinality()*poly_loop_check_that_candidates_have_question_and_that_it_isnt_trivial(f) + 2*poly_candidates_with_same_answer(f) + 2*poly_candidates_with_same_answer(g) + 2*iv.UBSize();
-    
-    f.UBSize() + 3 + f.Cardinality()*poly_loop_check_that_candidates_have_question_and_that_it_isnt_trivial(f) +
-      6*f.UBSize()*f.Cardinality() + 4*f.UBSize_Keys()*f.Cardinality() + 2*f.UBSize() + 2*f.Cardinality() + 6*g.UBSize()*g.Cardinality() + 4*g.UBSize_Keys()*g.Cardinality() + 2*g.UBSize() + 2*g.Cardinality() + 2*iv.UBSize() + 8;
-    
-    f.Cardinality()*poly_loop_check_that_candidates_have_question_and_that_it_isnt_trivial(f) +
-      6*f.UBSize()*f.Cardinality() + 7*f.UBSize() + 2*f.Cardinality() + 6*g.UBSize()*g.Cardinality() + 6*g.UBSize() + 2*g.Cardinality() + 2*iv.UBSize() + 11;
-    
-    f.Cardinality()*(f.UBSize() + 3*f.UBSize_Keys() + 1) +
-      6*f.UBSize()*f.Cardinality() + 7*f.UBSize() + 2*f.Cardinality() + 6*g.UBSize()*g.Cardinality() + 6*g.UBSize() + 2*g.Cardinality() + 2*iv.UBSize() + 11;
-    
-    f.UBSize()*f.Cardinality() + 3*f.UBSize() + f.Cardinality() +
-      6*f.UBSize()*f.Cardinality() + 7*f.UBSize() + 2*f.Cardinality() + 6*g.UBSize()*g.Cardinality() + 6*g.UBSize() + 2*g.Cardinality() + 2*iv.UBSize() + 11;
-    
-    7*f.UBSize()*f.Cardinality() + 10*f.UBSize() + 3*f.Cardinality() + 6*g.UBSize()*g.Cardinality() + 6*g.UBSize() + 2*g.Cardinality() + 2*iv.UBSize() + 11;
-  }
-  calc <= {
-    poly_verifyCDPC_base_case(f, g, P, iv) + f.UBSize() + 3 + f.Cardinality()*poly_loop_check_that_candidates_have_question_and_that_it_isnt_trivial(f) + 2*poly_candidates_with_same_answer(f) + 2*poly_candidates_with_same_answer(g) + 2*iv.UBSize();
-
-    poly_verifyCDPC_base_case(f, g, P, iv) +
-      7*f.UBSize()*f.Cardinality() + 10*f.UBSize() + 3*f.Cardinality() + 6*g.UBSize()*g.Cardinality() + 6*g.UBSize() + 2*g.Cardinality() + 2*iv.UBSize() + 11;
-
-    f.UBSize()*f.Cardinality()*P.Cardinality() + 3*f.UBSize()*P.Cardinality() + f.Cardinality()*P.Cardinality() + 2*f.UBSize()*f.Cardinality() + 2*f.UBSize() + f.Cardinality() + P.UBSize0()*P.Cardinality() + 3*P.Cardinality() + P.UBSize0() + 5 +
-      7*f.UBSize()*f.Cardinality() + 10*f.UBSize() + 3*f.Cardinality() + 6*g.UBSize()*g.Cardinality() + 6*g.UBSize() + 2*g.Cardinality() + 2*iv.UBSize() + 11;
-    
-    
-    f.UBSize()*f.Cardinality()*P.Cardinality() + 3*f.UBSize()*P.Cardinality() + f.Cardinality()*P.Cardinality()
-      + 9*f.UBSize()*f.Cardinality() + 12*f.UBSize() + 4*f.Cardinality() + 6*g.UBSize()*g.Cardinality() + 6*g.UBSize() + 2*g.Cardinality() + P.UBSize0()*P.Cardinality() + 3*P.Cardinality() + P.UBSize0()+ 2*iv.UBSize() + 16;
+    reveal pred_variables_inductive_step(f, g, P, a, b, x, y, iv, question, question_is_valid_and_not_trivial, f_true, g_true, iv_true, nodes_true, f_false, g_false, iv_false, nodes_false);
+    assert pred_variables_inductive_step(f, g, P, a, b, x, y, iv, question, question_is_valid_and_not_trivial, f_true, g_true, iv_true, nodes_true, f_false, g_false, iv_false, nodes_false);
   }
 
-  assert 0 <= poly_verifyCDPC_base_case(f, g, P, iv);
-  assert 0 <= f.UBSize() + 3 + f.Cardinality()*poly_loop_check_that_candidates_have_question_and_that_it_isnt_trivial(f) + 2*poly_candidates_with_same_answer(f) + 2*poly_candidates_with_same_answer(g) + 2*iv.UBSize();
+  ...
 
-  assert 0 <= 2*poly_candidates_with_same_answer(f) + 2*poly_candidates_with_same_answer(g) + 2*iv.UBSize();
+method verifyCDPC_inductive_step(f:Map_Map_T<int, bool, bool>, g:Map_Map_T<int, bool, int>, P:Set<int>, a:real, b:real, x:real, y:real, iv:Interview,
+                                 f_true:Map_Map_T<int, bool, bool>, g_true:Map_Map_T<int, bool, int>, iv_true:Interview,
+                                 f_false:Map_Map_T<int, bool, bool>, g_false:Map_Map_T<int, bool, int>, iv_false:Interview,
+                                 question:int, question_is_valid_and_not_trivial:bool, ghost nodes_true:nat, ghost nodes_false:nat,
+                                 ghost nodes:nat, ghost counter_in:nat)
+                                 returns (r:bool, ghost counter:nat)
+  decreases reveal pred_variables_inductive_step(f, g, P, a, b, x, y, iv, question, question_is_valid_and_not_trivial, f_true, g_true, iv_true, nodes_true, f_false, g_false, iv_false, nodes_false); nodes
+  requires (nodes_true < nodes) && (nodes_false < nodes)
 
-  f.UBSize()*f.Cardinality()*P.Cardinality() + 3*f.UBSize()*P.Cardinality() + f.Cardinality()*P.Cardinality()
-  + 9*f.UBSize()*f.Cardinality() + 12*f.UBSize() + 4*f.Cardinality() + 6*g.UBSize()*g.Cardinality() + 6*g.UBSize() + 2*g.Cardinality() + P.UBSize0()*P.Cardinality() + 3*P.Cardinality() + P.UBSize0()+ 2*iv.UBSize() + 16
-}
+  requires pred_problem_preconditions(f, g, P, a, b, x, y, iv)
+  requires pred_branch_info(iv, question_is_valid_and_not_trivial, question)
+  requires pred_variables_inductive_step(f, g, P, a, b, x, y, iv, question, question_is_valid_and_not_trivial, f_true, g_true, iv_true, nodes_true, f_false, g_false, iv_false, nodes_false)
 
-ghost function poly_verifyCDPC_base_case(f:Map_Map_T<int, bool, bool>, g:Map_Map_T<int, bool, int>, P:Set<int>, iv:Interview) : (o:nat)
-  ensures poly_correct_apt_ratio(f) + poly_correct_private_ratio(f, P) + 2 <= o
+  ensures reveal pred_problem_preconditions(f, g, P, a, b, x, y, iv); r == certificateCDPC(f.Model(), g.Model(), P.Model(), a, b, x, y, iv.Model())
+  ensures counter <= counter_in + nodes_true*poly_verifyCDPC_node(f_true, g_true, P, iv_true) + nodes_false*poly_verifyCDPC_node(f_false, g_false, P, iv_false)
 {
-  f.UBSize()*f.Cardinality()*P.Cardinality() + 3*f.UBSize()*P.Cardinality() + f.Cardinality()*P.Cardinality() + 2*f.UBSize()*f.Cardinality() + 2*f.UBSize() + f.Cardinality() + P.UBSize0()*P.Cardinality() + 3*P.Cardinality() + P.UBSize0() + 4
-}
-
-ghost function poly_loop_check_that_candidates_have_question_and_that_it_isnt_trivial<T>(f:Map_Map_T<int, bool, T>) : (o:nat)
-{
-  f.UBSize() + 3*f.UBSize_Keys() + 1
-}
-
-ghost function poly_correct_apt_ratio<T>(f:Map_Map_T<int, bool, T>) : (o:nat)
-  ensures f.UBSize() + 1 + f.Cardinality()*poly_correct_apt_ratio_loop(f) <= o
-{
-  /*calc == {
-    f.UBSize() + 1 + f.Cardinality()*poly_correct_apt_ratio_loop(f);
-    f.UBSize() + 1 + f.Cardinality()*(2*f.UBSize() + f.UBSize_Keys() + 1);
-    f.UBSize() + 1 + (2*f.UBSize()*f.Cardinality() + f.UBSize_Keys()*f.Cardinality() + f.Cardinality());
-    f.UBSize() + 1 + (2*f.UBSize()*f.Cardinality() + f.UBSize() + f.Cardinality());
-    2*f.UBSize()*f.Cardinality() + 2*f.UBSize() + f.Cardinality() + 1;
-  }*/
-  2*f.UBSize()*f.Cardinality() + 2*f.UBSize() + f.Cardinality() + 1
-}
-
-ghost function poly_correct_apt_ratio_loop<T>(f:Map_Map_T<int, bool, T>) : (o:nat)
-{
-  2*f.UBSize() + f.UBSize_Keys() + 1
-}
-
-ghost function poly_correct_private_ratio<T>(f:Map_Map_T<int, bool, T>, P:Set<int>) : (o:nat)
-  ensures P.UBSize0() + 1 + P.Cardinality()*poly_correct_private_ratio_outer_loop(f, P) <= o
-{
-  /*calc == {
-    P.UBSize0() + 1 + P.Cardinality()*poly_correct_private_ratio_outer_loop(f, P);
-    P.UBSize0() + 1 + P.Cardinality()*(f.UBSize()*f.Cardinality() + 3*f.UBSize() + f.Cardinality() + P.UBSize0() + 3);
-    P.UBSize0() + 1 + (f.UBSize()*f.Cardinality()*P.Cardinality() + 3*f.UBSize()*P.Cardinality() + f.Cardinality()*P.Cardinality() + P.UBSize0()*P.Cardinality() + 3*P.Cardinality());
-    f.UBSize()*f.Cardinality()*P.Cardinality() + 3*f.UBSize()*P.Cardinality() + f.Cardinality()*P.Cardinality() + P.UBSize0()*P.Cardinality() + 3*P.Cardinality() + P.UBSize0() + 1;
-  }*/
-  f.UBSize()*f.Cardinality()*P.Cardinality() + 3*f.UBSize()*P.Cardinality() + f.Cardinality()*P.Cardinality() + P.UBSize0()*P.Cardinality() + 3*P.Cardinality() + P.UBSize0() + 1
-}
-
-ghost function poly_correct_private_ratio_outer_loop<T>(f:Map_Map_T<int, bool, T>, P:Set<int>) : (o:nat)
-  ensures f.UBSize() + P.UBSize0() + 3 + f.Cardinality()*poly_correct_private_ratio_inner_loop(f) <= o
-{
-  /*calc == {
-    f.UBSize() + P.UBSize0() + 3 + f.Cardinality()*poly_correct_private_ratio_inner_loop(f);
-    f.UBSize() + P.UBSize0() + 3 + f.Cardinality()*(f.UBSize() + 2*f.UBSize_Keys() + 1);
-    f.UBSize() + P.UBSize0() + 3 + (f.UBSize()*f.Cardinality() + 2*f.UBSize_Keys()*f.Cardinality() + f.Cardinality());
-    f.UBSize() + f.UBSize()*f.Cardinality() + 2*f.UBSize_Keys()*f.Cardinality() + f.Cardinality() + P.UBSize0() + 3;
-    f.UBSize() + f.UBSize()*f.Cardinality() + 2*f.UBSize() + f.Cardinality() + P.UBSize0() + 3;
-    f.UBSize()*f.Cardinality() + 3*f.UBSize() + f.Cardinality() + P.UBSize0() + 3;
-  }*/
-  f.UBSize()*f.Cardinality() + 3*f.UBSize() + f.Cardinality() + P.UBSize0() + 3
-}
-
-ghost function poly_correct_private_ratio_inner_loop<T>(f:Map_Map_T<int, bool, T>) : (o:nat)
-{
-  f.UBSize() + 2*f.UBSize_Keys() + 1
-}
-
-ghost function poly_candidates_with_same_answer<T>(f:Map_Map_T<int, bool, T>) : (o:nat)
-{
-  /*calc == {
-    f.UBSize() + 2 + f.Cardinality()*poly_candidates_with_same_answer_loop(f);
-    f.UBSize() + 2 + f.Cardinality()*(3*f.UBSize() + 2*f.UBSize_Keys() + 1);
-    f.UBSize() + 2 + (3*f.UBSize()*f.Cardinality() + 2*f.UBSize_Keys()*f.Cardinality() + f.Cardinality());
-    3*f.UBSize()*f.Cardinality() + 2*f.UBSize_Keys()*f.Cardinality() + f.UBSize() + f.Cardinality() + 2;
-  }*/
-  3*f.UBSize()*f.Cardinality() + 2*f.UBSize_Keys()*f.Cardinality() + f.UBSize() + f.Cardinality() + 2
-}
-
-ghost function poly_candidates_with_same_answer_loop<T>(f:Map_Map_T<int, bool, T>) : (o:nat)
-{
-  3*f.UBSize() + 2*f.UBSize_Keys() + 1
-}
-
-
-
-
-
-// LEMMAS
-
-
-
-
-
-lemma lemma_card_apt_set_when_remove_element(f:map<candidate, bool>, cands:set<candidate>, cand:candidate)
-  requires cand in cands
-  requires cands <= f.Keys
-  ensures if f[cand] then
-            (|(set aptCand:candidate | aptCand in cands && f[aptCand] :: aptCand)|
-            ==
-            |(set aptCand:candidate | aptCand in (cands - {cand}) && f[aptCand] :: aptCand)| + 1)
-          else
-            |(set aptCand:candidate | aptCand in cands && f[aptCand] :: aptCand)|
-            ==
-            |(set aptCand:candidate | aptCand in (cands - {cand}) && f[aptCand] :: aptCand)|
-{
-  if f[cand] {
-    assert (set aptCand:candidate | aptCand in (cands - {cand}) && f[aptCand] :: aptCand) + {cand}
-            ==
-            (set aptCand:candidate | aptCand in cands && f[aptCand] :: aptCand);
+  counter := counter_in;
+  var recursive_true:bool; recursive_true, counter := verifyCDPC_rec(f_true, g_true, P, a, b, x, y, iv_true, nodes_true, counter) by {
+    reveal pred_problem_preconditions(f, g, P, a, b, x, y, iv);
+    reveal pred_branch_info(iv, question_is_valid_and_not_trivial, question);
+    reveal pred_variables_inductive_step(f, g, P, a, b, x, y, iv, question, question_is_valid_and_not_trivial, f_true, g_true, iv_true, nodes_true, f_false, g_false, iv_false, nodes_false);
+    reveal pred_nodes(iv_true, nodes_true);
+    assert 0 < nodes_true by {
+      assert (exists c:candidate | c in f.Keys() :: c[question] == true);
+      ghost var cand_true :| cand_true in f.Keys() && cand_true[question] == true;
+      assert f_true.Model() == (map c:candidate | c in f.Keys() && c[question] == true :: f.Model()[c]);
+      assert cand_true in f_true.Model();
+      assert 1 <= f_true.Cardinality();
+      assert 0 <= |iv_true.Questions()|;
+      mult_preserves_order(0, 1, |iv_true.Questions()|, f_true.Cardinality());
+    }
+    assert nodes_true < nodes;
   }
-  else {
-    assert (set aptCand:candidate | aptCand in (cands - {cand}) && f[aptCand] :: aptCand)
-            ==
-            (set aptCand:candidate | aptCand in cands && f[aptCand] :: aptCand);
+  var recursive_false:bool; recursive_false, counter := verifyCDPC_rec(f_false, g_false, P, a, b, x, y, iv_false, nodes_false, counter) by {
+    reveal pred_problem_preconditions(f, g, P, a, b, x, y, iv);
+    reveal pred_branch_info(iv, question_is_valid_and_not_trivial, question);
+    reveal pred_variables_inductive_step(f, g, P, a, b, x, y, iv, question, question_is_valid_and_not_trivial, f_true, g_true, iv_true, nodes_true, f_false, g_false, iv_false, nodes_false);
+    reveal pred_nodes(iv_true, nodes_true);
+    assert 0 < nodes_false  by {
+      assert (exists c:candidate | c in f.Keys() :: c[question] == false);
+      ghost var cand_false :| cand_false in f.Keys() && cand_false[question] == false;
+      assert f_false.Model() == (map c:candidate | c in f.Keys() && c[question] == false :: f.Model()[c]);
+      assert cand_false in f_false.Model();
+      assert 1 <= f_false.Cardinality();
+      assert 0 <= |iv_false.Questions()|;
+      mult_preserves_order(0, 1, |iv_false.Questions()|, f_false.Cardinality());
+    }
+    assert nodes_false < nodes;
   }
-}
-
-
-lemma lemma_card_priv_set_when_remove_element(f:map<candidate, bool>, cands:set<candidate>, cand:candidate, p:int)
-  requires cand in cands
-  requires cands <= f.Keys
-  requires forall c:candidate | c in f.Keys :: p in c.Keys
-  ensures if cand[p] then
-            (|(set privCand:candidate | privCand in cands && privCand[p] :: privCand)|
-            ==
-            |(set privCand:candidate | privCand in (cands - {cand}) && privCand[p] :: privCand)| + 1)
-          else
-            |(set privCand:candidate | privCand in cands && privCand[p] :: privCand)|
-            ==
-            |(set privCand:candidate | privCand in (cands - {cand}) && privCand[p] :: privCand)|
-{
-  if cand[p] {
-    assert (set privCand:candidate | privCand in (cands - {cand}) && privCand[p] :: privCand) + {cand}
-            ==
-            (set privCand:candidate | privCand in cands && privCand[p] :: privCand);
-  }
-  else {
-    assert (set privCand:candidate | privCand in (cands - {cand}) && privCand[p] :: privCand)
-            ==
-            (set privCand:candidate | privCand in cands && privCand[p] :: privCand);
-  }
-}
-
-
-
-lemma lemma_private_ratio(f:Map_Map_T<int, bool, bool>, P:Set<int>, P':Set<int>, P'':Set<int>, a:real, b:real, r:bool, r':bool, p:int, privateRatio:real)
-  requires f.Valid()
-  requires forall c1, c2:candidate |  c1 in f.Keys() && c2 in f.Keys() :: c1.Keys == c2.Keys
-  requires 0.0 <= a <= b <= 1.0
-  requires forall c:candidate | c in f.Keys() :: (P.Model() <= c.Keys)
-  requires f.Cardinality() != 0
-
-  requires in_universe_Set(P', P)
-  requires P'.Cardinality() != 0
-  requires r == forall p:int | p in (P.Model() - P'.Model()) ::
-              (
-                var privateRatio:real := (|(set isPrivate:candidate | isPrivate in f.Keys() && isPrivate[p] :: isPrivate)| as real) / (f.Cardinality() as real);
-                a <= privateRatio <= b
-              )
+  r := question_is_valid_and_not_trivial && recursive_true && recursive_false;
+  assert counter <= counter_in + poly_verifyCDPC_node(f, g, P, iv) + nodes_true*poly_verifyCDPC_node(f_true, g_true, P, iv_true) + nodes_false*poly_verifyCDPC_node(f_false, g_false, P, iv_false);
   
-
-  requires P'.Model() == (P''.Model() + {p})
-  requires p !in P''.Model()
-  requires privateRatio == (|(set isPrivate:candidate | isPrivate in f.Keys() && isPrivate[p] :: isPrivate)| as real) / (f.Cardinality() as real)
-  requires r' == (r && (a <= privateRatio <= b))
-
-  ensures r' == forall p:int | p in (P.Model() - P''.Model()) ::
-              (
-                var privateRatio:real := (|(set isPrivate:candidate | isPrivate in f.Keys() && isPrivate[p] :: isPrivate)| as real) / (f.Cardinality() as real);
-                a <= privateRatio <= b
-              )
-
-{
-  assert r == forall p:int | p in (P.Model() - P'.Model()) ::
-              (
-                var privateRatio:real := (|(set isPrivate:candidate | isPrivate in f.Keys() && isPrivate[p] :: isPrivate)| as real) / (f.Cardinality() as real);
-                a <= privateRatio <= b
-              );
-  assert r' == ((forall p:int | p in (P.Model() - P'.Model()) ::
-              (
-                var privateRatio:real := (|(set isPrivate:candidate | isPrivate in f.Keys() && isPrivate[p] :: isPrivate)| as real) / (f.Cardinality() as real);
-                a <= privateRatio <= b
-              ))
-              &&
-              (a <= privateRatio <= b))
-              ;
-  assert (P.Model() - P''.Model()) == ((P.Model() - P'.Model()) + {p});
-}
-
-
-
-lemma candidates_with_same_answer_lemma_1<T>(f:Map_Map_T<int, bool, T>, f':Map_Map_T<int, bool, T>,  f'':Map_Map_T<int, bool, T>, f'_out:Map_Map_T<int, bool, T>, f''_out:Map_Map_T<int, bool, T>, cand:Map<int, bool>, question:int, answer:bool)
-  requires forall c1, c2:candidate |  c1 in f.Keys() && c2 in f.Keys() :: c1.Keys == c2.Keys
-  requires forall c:candidate |  c in f.Keys() :: question in c
-  requires in_universe_Map_Map_T(f', f)
-  requires in_universe_Map_Map_T(f'', f)
-  requires f'.Cardinality() != 0
-  requires f''.Model() == (map c:candidate | c in (f.Keys() - f'.Keys()) && c[question] == answer :: f.Model()[c])
-
-  requires f'_out.Keys() == f'.Keys() - {cand.Model()}
-  requires cand.Model() in f'.Model()
-  requires cand.Model()[question] == answer
-  requires f''_out.Model() == f''.Model()[cand.Model() := f.Model()[cand.Model()]]
-
-  ensures f''_out.Model() == (map c:candidate | c in (f.Keys() - f'_out.Keys()) && c[question] == answer :: f.Model()[c])
-{
-  assert f''_out.Model() == (map c:candidate | c in (f.Keys() - f'.Keys()) && c[question] == answer :: f.Model()[c])[cand.Model() := f.Model()[cand.Model()]];
-  candidates_with_same_answer_lemma_1_aux(f, f', cand, question, answer);
-  assert f''_out.Model() == (map c:candidate | c in (f.Keys() - f'.Keys() + {cand.Model()}) && c[question] == answer :: f.Model()[c]);
-
-  assert f'_out.Keys() == f'.Keys() - {cand.Model()};
-  assert (f.Keys() - f'.Keys() + {cand.Model()}) == (f.Keys() - f'_out.Keys());
-}
-
-
-lemma candidates_with_same_answer_lemma_2<T>(f:Map_Map_T<int, bool, T>, f':Map_Map_T<int, bool, T>,  f'':Map_Map_T<int, bool, T>, f'_out:Map_Map_T<int, bool, T>, f''_out:Map_Map_T<int, bool, T>, cand:Map<int, bool>, question:int, answer:bool)
-  requires forall c1, c2:candidate |  c1 in f.Keys() && c2 in f.Keys() :: c1.Keys == c2.Keys
-  requires forall c:candidate |  c in f.Keys() :: question in c
-  requires in_universe_Map_Map_T(f', f)
-  requires in_universe_Map_Map_T(f'', f)
-  requires f'.Cardinality() != 0
-  requires f''.Model() == (map c:candidate | c in (f.Keys() - f'.Keys()) && c[question] == answer :: f.Model()[c])
-
-  requires f'_out.Keys() == f'.Keys() - {cand.Model()}
-  requires cand.Model() in f'.Model()
-  requires cand.Model()[question] != answer
-  requires f''_out.Model() == f''.Model()
-
-  ensures f''_out.Model() == (map c:candidate | c in (f.Keys() - f'_out.Keys()) && c[question] == answer :: f.Model()[c])
-{
-  assert f''_out.Model() == f''.Model();
-  assert f''_out.Model() == (map c:candidate | c in (f.Keys() - f'.Keys()) && c[question] == answer :: f.Model()[c]);
-  candidates_with_same_answer_lemma_2_aux(f, f'_out, cand, question, answer);
-  assert f''_out.Model() == (map c:candidate | c in (f.Keys() - f'_out.Keys() - {cand.Model()}) && c[question] == answer :: f.Model()[c]);
-  assert forall c:candidate | c in (f.Keys() - f'_out.Keys() - {cand.Model()}) && c[question] == answer :: c !in {cand.Model()};
-  assert forall c:candidate | c in (f.Keys() - f'_out.Keys() - {cand.Model()}) && c[question] == answer :: c in (f.Keys() - f'_out.Keys());
-
-  assert (map c:candidate | c in (f.Keys() - f'_out.Keys() - {cand.Model()}) && c[question] == answer :: f.Model()[c]) ==
-          (map c:candidate | c in (f.Keys() - f'_out.Keys()) && c[question] == answer :: f.Model()[c]);
-}
- 
-
-lemma candidates_with_same_answer_lemma_1_aux<T>(f:Map_Map_T<int, bool, T>, f':Map_Map_T<int, bool, T>, cand:Map<int, bool>, question:int, answer:bool)
-  requires forall c:candidate |  c in f.Keys() :: question in c
-  requires cand.Model() in f.Model()
-  requires cand.Model()[question] == answer
-
-  ensures 
-          (map c:candidate | c in (f.Keys() - f'.Keys()) && c[question] == answer :: f.Model()[c])[cand.Model() := f.Model()[cand.Model()]]
-          ==
-          (map c:candidate | c in (f.Keys() - f'.Keys() + {cand.Model()}) && c[question] == answer :: f.Model()[c])
-{}
-
-lemma candidates_with_same_answer_lemma_2_aux<T>(f:Map_Map_T<int, bool, T>, f'_out:Map_Map_T<int, bool, T>, cand:Map<int, bool>, question:int, answer:bool)
-  requires forall c:candidate |  c in f.Keys() :: question in c
-  requires cand.Model() in f.Model()
-  requires cand.Model()[question] != answer
-
-  ensures (map c:candidate | c in (f.Keys() - f'_out.Keys() - {cand.Model()}) && c[question] == answer :: f.Model()[c]) ==
-          (map c:candidate | c in (f.Keys() - f'_out.Keys()) && c[question] == answer :: f.Model()[c])
-{}
-
-lemma candidates_with_same_answer_restore_counter_invariant<T>(f:Map_Map_T<int, bool, T>, f':Map_Map_T<int, bool, T>, f'_prev:Map_Map_T<int, bool, T>, counter:nat, counter_in:nat)
-  requires counter <= counter_in + f.UBSize() + 2 + (f.Cardinality() - f'_prev.Cardinality())*poly_candidates_with_same_answer_loop(f) + poly_candidates_with_same_answer_loop(f)
-  requires f'_prev.Cardinality() == (f'.Cardinality() + 1)
-  ensures counter <= counter_in + f.UBSize() + 2 + (f.Cardinality() - f'.Cardinality())*poly_candidates_with_same_answer_loop(f)
-{
-  /*assert (f.Cardinality() - f'_prev.Cardinality()) == (f.Cardinality() - (f'.Cardinality() + 1));
-  assert (f.Cardinality() - f'_prev.Cardinality())*poly_candidates_with_same_answer_loop(f) == (f.Cardinality() - (f'.Cardinality() + 1))*poly_candidates_with_same_answer_loop(f);
-  assert counter <= counter_in + f.UBSize() + 2 + (f.Cardinality() - (f'.Cardinality() + 1))*poly_candidates_with_same_answer_loop(f) + poly_candidates_with_same_answer_loop(f);*/
-}
-
-lemma verifyCDPC_restore_counter_invariant<T>(f:Map_Map_T<int, bool, T>, f':Map_Map_T<int, bool, T>, f'_prev:Map_Map_T<int, bool, T>, counter:nat, counter_in:nat)
-  requires counter <= counter <= counter_in + f.UBSize() + 3 + (f.Cardinality() - f'_prev.Cardinality())*poly_loop_check_that_candidates_have_question_and_that_it_isnt_trivial(f) + poly_loop_check_that_candidates_have_question_and_that_it_isnt_trivial(f)
-  requires f'_prev.Cardinality() == (f'.Cardinality() + 1)
-  ensures counter <= counter_in + f.UBSize() + 3 + (f.Cardinality() - f'.Cardinality())*poly_loop_check_that_candidates_have_question_and_that_it_isnt_trivial(f)
-{}
-
-
-lemma verifyCDPC_restore_counter_base_case(f:Map_Map_T<int, bool, bool>, g:Map_Map_T<int, bool, int>, P:Set<int>, iv:Interview, nodes:nat, counter:nat, counter_in:nat)
-  requires pred_nodes(iv, f, nodes)
-  requires counter <= counter_in + poly_verifyCDPC_base_case(f, g, P, iv)
-  ensures counter <= counter_in + nodes*poly_verifyCDPC_node(f, g, P, iv)
-{
-  assert counter <= counter_in + poly_verifyCDPC_node(f, g, P, iv);
-  reveal pred_nodes(iv, f, nodes);
-  mult_preserves_order(1, poly_verifyCDPC_node(f, g, P, iv), nodes, poly_verifyCDPC_node(f, g, P, iv));
-  assert poly_verifyCDPC_node(f, g, P, iv) <= nodes*poly_verifyCDPC_node(f, g, P, iv);
-  assert counter <= counter_in + nodes*poly_verifyCDPC_node(f, g, P, iv);
-}
-
-
-lemma candidates_with_same_answer_counter_simplification<T>(f:Map_Map_T<int, bool, T>, f':Map_Map_T<int, bool, T>, counter:nat, counter_in:nat)
-  requires f'.Cardinality() == 0
-  requires counter <= counter_in + f.UBSize() + 2 + (f.Cardinality() - f'.Cardinality())*poly_candidates_with_same_answer_loop(f)
-  ensures counter <= counter_in + poly_candidates_with_same_answer(f)
-{
-  //identity_substraction_lemma(f.Keys(), f'.Keys());
-  //assert counter <= counter_in + f.UBSize() + 2 + f.Cardinality()*poly_candidates_with_same_answer_loop(f);
-}
-
-lemma postcondition_verifyCDPC(f:Map_Map_T<int, bool, bool>, g:Map_Map_T<int, bool, int>, P:Set<int>, a:real, b:real, x:real, y:real, iv:Interview, question:int, question_is_valid_and_not_trivial:bool, recursive_true:bool, recursive_false:bool, r:bool)
-  requires pred_problem_preconditions(f, g, P, a, b, x, y, iv)
-  requires pred_branch_info(iv, question_is_valid_and_not_trivial, question)
-  requires pred_variables_lemma(f, g, P, a, b, x, y, iv, question, question_is_valid_and_not_trivial, recursive_true, recursive_false, r)
-  ensures reveal pred_problem_preconditions(f, g, P, a, b, x, y, iv);
-          reveal pred_branch_info(iv, question_is_valid_and_not_trivial);
-          reveal pred_variables_lemma(f, g, P, a, b, x, y, iv, question, question_is_valid_and_not_trivial, recursive_true, recursive_false, r);
-          r == certificateCDPC(f.Model(), g.Model(), P.Model(), a, b, x, y, iv.Model())
-{
-  reveal pred_problem_preconditions(f, g, P, a, b, x, y, iv);
-  reveal pred_branch_info(iv, question_is_valid_and_not_trivial);
-  reveal pred_variables_lemma(f, g, P, a, b, x, y, iv, question, question_is_valid_and_not_trivial, recursive_true, recursive_false, r);
-}
-
-
-
-// Predicates
-
-
-
-ghost opaque predicate pred_problem_preconditions(f:Map_Map_T<int, bool, bool>, g:Map_Map_T<int, bool, int>, P:Set<int>, a:real, b:real, x:real, y:real, iv:Interview)
-{
-  (f.Valid() && g.Valid() && P.Valid() && iv.Valid()) &&
-  (forall c1, c2:candidate |  c1 in f.Keys() && c2 in f.Keys() :: c1.Keys == c2.Keys) &&
-  (f.Keys() == g.Keys()) &&
-  (forall c:candidate | c in f.Keys() :: (P.Model() <= c.Keys)) &&
-  (0.0 <= a <= b <= 1.0) &&
-  (0.0 <= x <= y <= 1.0)
-}
-
-ghost opaque predicate pred_nodes(iv:Interview, f:Map_Map_T<int, bool, bool>, nodes:nat)
-{
-  0 < nodes == |iv.Questions()|*f.Cardinality() + 1   // |iv.Questions()|*|iv.Candidates()| + 1
-}
-
-ghost opaque predicate pred_branch_info(iv:Interview, question_is_valid_and_not_trivial:bool, question:int)
-{
-  (iv.Model() != Null) &&
-  (question_is_valid_and_not_trivial == true) &&
-  (iv.Model().Key == question)
-}
-
-ghost opaque predicate pred_variables_lemma(f:Map_Map_T<int, bool, bool>, g:Map_Map_T<int, bool, int>, P:Set<int>, a:real, b:real, x:real, y:real, iv:Interview, question:int, question_is_valid_and_not_trivial:bool, recursive_true:bool, recursive_false:bool, ok:bool)
-  requires pred_problem_preconditions(f, g, P, a, b, x, y, iv)
-  requires pred_branch_info(iv, question_is_valid_and_not_trivial, question)
-{
-  reveal pred_problem_preconditions(f, g, P, a, b, x, y, iv); reveal pred_branch_info(iv, question_is_valid_and_not_trivial);
-  (question == iv.Model().Key) &&
-  (question_is_valid_and_not_trivial ==
-    ((forall cand:candidate | cand in f.Keys() :: question in cand.Keys) &&
-    (exists cand:candidate | cand in f.Keys() :: cand[question] == true) &&
-    (exists cand:candidate | cand in f.Keys() :: cand[question] == false))
-  ) &&
-  (recursive_true ==
-    certificateCDPC(
+  assert
+      (recursive_true == certificateCDPC(
       (map c:candidate | c in f.Keys() && c[question] == true :: f.Model()[c]),
       (map c:candidate | c in g.Keys() && c[question] == true :: g.Model()[c]),
       P.Model(), a, b, x, y, iv.Model().True
-    )
-  ) &&
-  (recursive_false ==
-    certificateCDPC(
+    ))
+    &&
+    (recursive_false == certificateCDPC(
       (map c:candidate | c in f.Keys() && c[question] == false :: f.Model()[c]),
       (map c:candidate | c in g.Keys() && c[question] == false :: g.Model()[c]),
       P.Model(), a, b, x, y, iv.Model().False
-    )
-  ) &&
-  (ok == (question_is_valid_and_not_trivial && recursive_true && recursive_false))
-}
+    ))
+  by {
+    reveal pred_problem_preconditions(f, g, P, a, b, x, y, iv);
+    reveal pred_branch_info(iv, question_is_valid_and_not_trivial, question);
+    reveal pred_variables_inductive_step(f, g, P, a, b, x, y, iv, question, question_is_valid_and_not_trivial, f_true, g_true, iv_true, nodes_true, f_false, g_false, iv_false, nodes_false);
+  }
 
-ghost opaque predicate pred_ok_definition(question_is_valid_and_not_trivial:bool, recursive_true:bool, recursive_false:bool, ok:bool)
-{
-  (ok == (question_is_valid_and_not_trivial && recursive_true && recursive_false))
-}
+  postcondition_verifyCDPC(f, g, P, a, b, x, y, iv, question, question_is_valid_and_not_trivial, recursive_true, recursive_false, r) by {
+    assert pred_variables_lemma(f, g, P, a, b, x, y, iv, question, question_is_valid_and_not_trivial, recursive_true, recursive_false, r) by {
+      reveal pred_variables_lemma(f, g, P, a, b, x, y, iv, question, question_is_valid_and_not_trivial, recursive_true, recursive_false, r);
+      reveal pred_branch_info(iv, question_is_valid_and_not_trivial, question);
+      reveal pred_variables_inductive_step(f, g, P, a, b, x, y, iv, question, question_is_valid_and_not_trivial, f_true, g_true, iv_true, nodes_true, f_false, g_false, iv_false, nodes_false);
+    }
+  }
 
-ghost opaque predicate pred_variables_inductive_step(f:Map_Map_T<int, bool, bool>, g:Map_Map_T<int, bool, int>, P:Set<int>, a:real, b:real, x:real, y:real, iv:Interview, question:int, question_is_valid_and_not_trivial:bool,
-                                                     f_true:Map_Map_T<int, bool, bool>, g_true:Map_Map_T<int, bool, int>, iv_true:Interview, nodes_true:nat,
-                                                     f_false:Map_Map_T<int, bool, bool>, g_false:Map_Map_T<int, bool, int>, iv_false:Interview, nodes_false:nat)
-  requires pred_problem_preconditions(f, g, P, a, b, x, y, iv)
-  requires pred_branch_info(iv, question_is_valid_and_not_trivial, question)
-{
-  reveal pred_problem_preconditions(f, g, P, a, b, x, y, iv); reveal pred_branch_info(iv, question_is_valid_and_not_trivial, question);
-  (f_true.Valid() && f_false.Valid() && g_true.Valid() && g_false.Valid() && iv_true.Valid() && iv_false.Valid()) &&
-  (question_is_valid_and_not_trivial == (
-    (forall cand:candidate | cand in f.Keys() :: question in cand.Keys) &&    // candidates have question
-    (exists cand:candidate | cand in f.Keys() :: cand[question] == true) &&   // exists answer true
-    (exists cand:candidate | cand in f.Keys() :: cand[question] == false))    // exists answer false
-  ) &&
-  (f_true.Model() == (map c:candidate | c in f.Keys() && c[question] == true :: f.Model()[c])) &&
-  (f_false.Model() == (map c:candidate | c in f.Keys() && c[question] == false :: f.Model()[c])) &&
-  (g_true.Model() == (map c:candidate | c in g.Keys() && c[question] == true :: g.Model()[c])) &&
-  (g_false.Model() == (map c:candidate | c in g.Keys() && c[question] == false :: g.Model()[c])) &&
-  ((iv_true.Model() == iv.Model().True) && iv_true.Questions() == iv.Questions() - {iv.Model().Key}) &&
-  ((iv_false.Model() == iv.Model().False) && iv_false.Questions() == iv.Questions() - {iv.Model().Key}) &&
-  (nodes_true == |iv_true.Questions()|*f_true.Cardinality() + 1) &&
-  (nodes_false == |iv_false.Questions()|*f_false.Cardinality() + 1)
+  return r, counter;
 }
+*/
 
